examples/tutorial/6-smt/tutorial_smtScript.sml
@@ -1,0 +1,99 @@
+open HolKernel Parse boolLib bossLib;
+
+(* From shared: *)
+open bir_exp_to_wordsLib bslSyntax;
+open pretty_exnLib;
+
+if !Globals.interactive then let
+  (* To simplify the life of our poor vim users *)
+  val _ = load "HolSmtLib";
+  val _ = load "tutorial_bir_to_armTheory";
+  val _ = load "tutorial_wpTheory";
+in () end else ();
+
+(* From examples: *)
+open tutorial_bir_to_armTheory;
+open tutorial_wpTheory;
+
+if !Globals.interactive then let
+  val _ = Parse.current_backend := PPBackEnd.vt100_terminal;
+  val _ = Globals.show_tags := true;
+  val _ = Globals.linewidth := 100;
+  val _ = Feedback.set_trace "HolSmtLib" 1;
+  val _ = bir_ppLib.install_bir_pretty_printers ();
+  (*
+  val _ = bir_ppLib.remove_bir_pretty_printers ();
+  val _ = Feedback.set_trace "HolSmtLib" 0;
+  val _ = Feedback.set_trace "HolSmtLib" 2;
+  val _ = Feedback.set_trace "HolSmtLib" 3;
+  val _ = Feedback.set_trace "HolSmtLib" 4;
+  *)
+in () end else ();
+
+val _ = new_theory "tutorial_smt";
+
+(* This function will prove `ante => conseq` using an SMT solver.
+ * If this fails, it will print a SAT model.
+ * 
+ * This function uses an oracle to create theorems about the generated
+ * words expression.
+ *)
+fun prove_imp_w_smt ante conseq =
+  let
+    val wrap_exn = Feedback.wrap_exn "tutorial_smt" "prove_imp_w_smt"
+    (* Create the implication as a BIR expression *)
+    val bir_impl = bor (bnot ante, conseq)
+      handle e => raise pp_exn_s
+        ( "Failed to create the implication. "
+        ^ "Make sure that `ante` and `conseq` are BIR expression terms.")
+        (wrap_exn e) 
+    val w_tm = bir2bool bir_impl
+    val proved_w_thm = HolSmtLib.Z3_ORACLE_PROVE w_tm
+      handle HOL_ERR e =>
+        let
+          fun print_model model = List.foldl
+            (fn ((name, tm), _) => (print (" - " ^ name ^ ": "); Hol_pp.print_term tm))
+            () (rev model);
+          val neg_tm = mk_neg w_tm
+          val model = Z3_SAT_modelLib.Z3_GET_SAT_MODEL neg_tm
+          val _ = print "Failed to prove the implication. Here is a counter-example:\n";
+          val _ = print_model model;
+        in
+          raise HOL_ERR e
+        end
+  in
+    proved_w_thm
+  end
+    handle e => raise pp_exn e;
+
+val EVALed_def_as_term = (rhs o concl o EVAL o rhs o concl)
+
+(******************     (1) bir_add_reg_entry      ********************)
+val contract_1_pre = EVALed_def_as_term bir_add_reg_contract_1_pre_def;
+val contract_1_wp  = EVALed_def_as_term bir_add_reg_entry_wp_def;
+val contract_1_imp = prove_imp_w_smt contract_1_pre contract_1_wp;
+
+(******************    (2)  bir_add_reg_loop     *********************)
+val contract_2_pre = EVALed_def_as_term bir_add_reg_contract_2_pre_def;
+val contract_2_wp  = EVALed_def_as_term bir_add_reg_loop_wp_def;
+val contract_2_imp = prove_imp_w_smt contract_2_pre contract_2_wp;
+
+(**************   (3)  bir_add_reg_loop_continue     *****************)
+val contract_3_pre = EVALed_def_as_term bir_add_reg_contract_3_pre_def;
+val contract_3_wp  = EVALed_def_as_term bir_add_reg_loop_continue_wp_def;
+val contract_3_imp = prove_imp_w_smt contract_3_pre contract_3_wp;
+
+(***************       bir_add_reg_loop_exit      *****************)
+val contract_4_pre = EVALed_def_as_term bir_add_reg_contract_4_pre_def;
+val contract_4_wp  = EVALed_def_as_term bir_add_reg_loop_exit_wp_def;
+val contract_4_imp = prove_imp_w_smt contract_4_pre contract_4_wp;
+
+val _ = List.map save_thm [
+  ("contract_1_imp", contract_1_imp),
+  ("contract_2_imp", contract_2_imp),
+  ("contract_3_imp", contract_3_imp),
+  ("contract_4_imp", contract_4_imp)
+];
+
+val _ = export_theory();
+
